<subsubsection xml:id="subsubsec-factorisation-when-the-coefficient-of-x-squared-is-one" xmlns:xi="http://www.w3.org/2001/XInclude">
    <title>Factorisation When The Coefficient Of <m>x^2</m> Is One</title>
    <p xml:id="auto_dp73d5r0">
        The expression
        <me>
            ax^2 + bx + c,
        </me>
        where <m>a, b, c</m> are constants and <m>a \neq 0</m>, is called a quadratic expression.
    </p>
    <p xml:id="auto_eyjfk2xh">
        In such expressions <m>a</m> is called the coefficient of <m>x^2</m>, <m>b</m> is called the coefficient of <m>x</m> and <m>c</m> is called the constant term.
    </p>
    <p xml:id="auto_kmekc0hk">
        When the coefficient of <m>x^2</m> is one, the expression is of the form;
        <me>
            x^2 + bx + c.
        </me>
    </p>
    <p xml:id="auto_hvjoe6cl">
        Cosider the following expressions:
        
    </p>
    <sidebyside>
    <p xml:id="auto_k6zseta3">
        <me>
            \text{(a).} \, (x + 3)(x + 4).
        </me>
    </p>
    <p xml:id="auto_26ypz13r">            
        <me>
           \text{(b).} \, (x -6)(x - 5).
        </me>                
    </p>
    </sidebyside>
    <sidebyside>
        <p xml:id="auto_ja7aehx1">
            Expanding the expressions we get:               
            <md>
                <mrow>(x + 3)(x + 4) \amp = x(x + 3) + 4(x + 3) </mrow>
            </md>
            <md>
                <mrow>(x + 3)(x + 4) \amp = x^2 + 3x + 4x + 12 </mrow>
            </md>
            Collecting like terms to get:
            <me>
                x^2 + 7x + 12.
            </me>
        </p>
        <p xml:id="auto_5lpsd36p">
            <m>\,</m>
        </p>
    <p xml:id="auto_xdse0lpa">
        Expanding the expressions we get:
        <md>
            <mrow>(x - 6)(x - 5) \amp = x(x - 5) - 6(x - 5) </mrow>
        </md>
        <md>
            <mrow>(x - 6)(x - 5) \amp = x^2 - 5x - 6x + 30 </mrow>
        </md>
        Simplify the middle terms:
        <me>
            x^2 - 11x + 30.
        </me>
    </p>
    </sidebyside>
    
    <p xml:id="auto_cn640cin">
        From the above examples, we can see that the expressions <m>x^2 + 7x + 12</m> and <m>x^2 - 11x + 30</m> are formed from the factors of expressions <m>(x + 3)(x + 4)</m> and <m>(x - 6)(x - 5)</m> respectively.
    </p>
    <p xml:id="auto_bge1pybj">
        The factorised form of the expression <m>x^2 + bx + c</m> is <m>(x + m)(x + n)</m> where <m>m</m> and <m>n</m> are the factors of <m>c</m> whose sum is <m>b</m>.
    </p>
    <p xml:id="auto_rvpg68qv">
        In each case;
        <ol xml:id="auto_qbepzv8i" marker="i">
            <li xml:id="auto_ug26ym22">
                <p xml:id="auto_0rkvaefj">
                    The sum of the constant terms in the factors is equal to the coefficient of <m>x</m> in the expression.
                </p>
            </li>
            <li xml:id="auto_fwl91cd1">
                <p xml:id="auto_7bow7r0y">
                    The product of the constant terms in the factors is equal to the constant term in the expression.
                </p>
            </li>
        </ol>
    </p>

    <example xml:id="auto_yrl3h9s0">
        <statement>
            <p xml:id="auto_mgkno0sg">
                
            </p>
            <p xml:id="auto_wssgp0pk">
                Factorise the following expression:
                <me>
                    x^2 + 5x + 6.
                </me>
            </p>
        </statement>
        <solution>
            <p xml:id="auto_ayw868ip">
                In this case, the coefficient of <m>x^2</m> is one, the coefficient of <m>x</m> is 5 and the constant term is 6.
            </p>
            <p xml:id="auto_ufbderfr">
                So the factors will be of the form <m>(x + m)(x + n)</m> where <m>m</m> and <m>n</m> are the factors of 6 whose sum is 5.
            </p>
            <p xml:id="auto_9rzvlze2">
                In the expression <m>x^2 + 5x + 6</m>, look for two numbers such the numbers <m>a</m> and <m>b</m> such that 
                <me>a + b = 5</me> is coefficient of <m>x</m> and <m>ab = 6</m> is the constant term.
            </p>
            <p xml:id="auto_33r4n2vz">
                In this case, the numbers are 2 and 3.
            </p>
            <p xml:id="auto_bojq5qrm">
                <me>
                    x^2 + 5x + 6 = x^2 + 2x + 3x + 6.
                </me>                
            </p>
            <p xml:id="auto_7r8scwv4">
                Grouping terms, we get:
            </p>
            <p xml:id="auto_w08tg6un">
                <me>
                    x^2 + 5x + 6 = x(x + 2) + 3(x + 2). <!-- Grouping terms -->
                </me>
            </p>
            <p xml:id="auto_j4jtwh8a">
                <me>
                    x^2 + 5x + 6 = (x + 2)(x + 3).
                </me>
            </p>
            <p xml:id="auto_294mn8zi">
                Therefore, the factorised form of the expression <m>x^2 + 5x + 6</m> is <m>(x + 2)(x + 3)</m>.
            </p>
        </solution>
    </example>

    <example xml:id="auto_y55gwt1n">
        <statement>
            <p xml:id="auto_lfloruyg">
                
            </p>
            <p xml:id="auto_g8ypuoew">
                Factorise the following expression:
                <me>
                    x^2 - 9x + 20.
                </me>
            </p>
        </statement>
        <solution>
            <p xml:id="auto_3r83c8me">
                Look for two numbers such that the numbers <m>a</m> and <m>b</m> such that <m>a + b = -9</m> and <m>ab = 20</m>.
            </p>
            <p xml:id="auto_3rl3xhl7">
                The numbers are -4 and -5.
            </p>
            <p xml:id="auto_0s2trovc">
                Then, the expression <m>x^2 - 9x + 20</m> can be written as:
                <me>
                    x^2 - 4x - 5x + 20.
                </me>                
            </p>
            <p xml:id="auto_ht8kos7u">
                Grouping terms, we get:
                <me>
                    x^2 - 9x + 20 = x(x - 4) - 5(x - 4).
                </me>                
            </p>
            <p xml:id="auto_ld1heie0">
                <me>
                    x^2 - 9x + 20 = (x - 4)(x - 5).
                </me>
            </p>
            <p xml:id="auto_hdkv36vm">
                The factorised form of the expression <m>x^2 - 9x + 20</m> is <m>(x - 4)(x - 5)</m>.
            </p>
        </solution>
    </example>

    <example xml:id="auto_7vmdrnv7">
        <statement>
            <p xml:id="auto_wsgwtp0e">
                
            </p>
            <p xml:id="auto_u8y3zind">
                Factorise the following expression:
                <me>
                    x^2 + 6x + 9.
                </me>
            </p>
        </statement>
        <solution>
            <p xml:id="auto_o0jum3kk">
                Look for two numbers such that the numbers <m>a</m> and <m>b</m> such that <m>a + b = 6</m> and <m>ab = 9</m>.
            </p>
            <p xml:id="auto_hrptcxzo">
                The numbers are 3 and 3.
            </p>
            <p xml:id="auto_cuz5fk9t">
                Then, the expression <m>x^2 + 6x + 9</m> can be written as:
                <me>
                    x^2 + 3x + 3x + 9.
                </me>
            </p>
            <p xml:id="auto_zygep1u9">
                Grouping terms, we get:
                <me>
                    x^2 + 6x + 9 = x(x + 3) + 3(x + 3).
                </me>
            </p>
            <p xml:id="auto_vxv0bqrv">
                <me>
                    x^2 + 6x + 9 = (x + 3)(x + 3).
                </me>
            </p>
            <p xml:id="auto_wk4dgwqp">
                The factorised form of the expression <m>x^2 + 6x + 9</m> is <m>(x + 3)(x + 3)</m>.
            </p>
        </solution>
    </example>

    <exercises xml:id="exercises-when-cofficient-of-x-squared-is-one">
        <exercise xml:id="auto_efnrotnf">
            <statement>
                <p xml:id="auto_uug3fpeh">
                    Factorise the following expressions:
                    <ol xml:id="auto_qb9ysrlw" marker="(a)." cols="3">
                        <li xml:id="auto_lak6jvxn">
                            <p xml:id="auto_vn5sovja">
                                <m>
                                    x^2 + 4x + 4.
                                </m>
                            </p>
                        </li>
                        <li xml:id="auto_cv4lswko">
                            <p xml:id="auto_pzlunqie">
                                <m>
                                    x^2 + 8x + 15.
                                </m>
                            </p>
                        </li>
                        <li xml:id="auto_2vmawb3e">
                            <p xml:id="auto_ldm0dfev">
                                <m>
                                    x^2 - 7x + 12.
                                </m>
                            </p>
                        </li>
                        <li xml:id="auto_qtlv2j9s">
                            <p xml:id="auto_b4u3ihm6">
                                <m>
                                    x^2 - 6x + 9.
                                </m>
                            </p>
                        </li>
                        <li xml:id="auto_01e4b0w2">
                            <p xml:id="auto_l6vv8u4z">
                                <m>
                                    x^2 + 3x + 2.
                                </m>
                            </p>
                        </li>
                        <li xml:id="auto_cr7a2xnb">
                            <p xml:id="auto_dajblsdz">
                                <m>
                                    x^2 - 5x + 6.
                                </m>
                            </p>
                        </li>
                        <li xml:id="auto_u91khnzo">
                            <p xml:id="auto_2edn7rz0">
                                <m>
                                    x^2 + 2x - 15.
                                </m>
                            </p>
                        </li>
                        <li xml:id="auto_s4838u0g">
                            <p xml:id="auto_aq8rkm9j">
                                <m>
                                    x^2 - 4x - 5.
                                </m>
                            </p>
                        </li>
                        <li xml:id="auto_zwl1kdbu">
                            <p xml:id="auto_lzlwybni">
                                <m>
                                    x^2 - 3x - 10.
                                </m>
                            </p>
                        </li>
                        <li xml:id="auto_ps0n5siv">
                            <p xml:id="auto_2abvrknj">
                                <m>
                                    x^2 + 7x + 10.
                                </m>
                            </p>
                        </li>
                        <li xml:id="auto_arqnj7z1">
                            <p xml:id="auto_6d1azi6c">
                                <m>
                                    x^2 - 8x - 20.
                                </m>
                            </p>
                        </li>
                        <li xml:id="auto_bwn7cjw6">
                            <p xml:id="auto_z96jygir">
                                <m>
                                    x^2 + 9x + 20.
                                </m>
                            </p>
                        </li>
                    </ol>
                </p>
            </statement>
        </exercise>
    </exercises>
</subsubsection>