<subsubsection xml:id="subsubsec-factorisation-when-the-coefficient-of-x-squared-is-not-one" xmlns:xi="http://www.w3.org/2001/XInclude">
    <title>Factorisation When The Coefficient Of <m>x^2</m> Is Not One.</title>
    <p xml:id="auto_rmt435zm">
        The general form of a quadratic expression is <m>ax^2 + bx + c</m>, where <m>a</m>, <m>b</m> and <m>c</m> are constants. 
    </p>
    <p xml:id="auto_yq19qlj5">
        In this section we are going to discuss how to factorise a quadratic expression when the <m>a</m> in <m>ax^2 + bx + c</m> is not equal to <m>1</m>.
    </p>
    <p xml:id="auto_7s7yws8j">
        Consider the following identities:
        <ol xml:id="auto_j9gxugoe" marker="(a)">
            <li xml:id="auto_wchkvdub">
                <p xml:id="auto_9lnt7bsz">
                    <m>(3x + 2)(2x + 1)</m>
                </p>
                <p xml:id="auto_npf2wo6x">
                    <me>
                        = (3x \times 2x) + (3x \times 1) + (2 \times 2x) + (2 \times 1)
                    </me>                    
                </p>
                <p xml:id="auto_s8r9qhcv">
                    <me>
                        = 6x^2 + 3x + 4x + 2
                    </me>                    
                </p>
                <p xml:id="auto_jtuvhbxv">
                    <me>
                        = 6x^2 + 7x + 2
                    </me>                    
                </p>
            </li>
            <li xml:id="auto_4q52sb2g">
                <p xml:id="auto_vawtfjvf">
                    <m>(3x - 2)(4x - 3)</m>
                </p>
                <p xml:id="auto_kggqgxoe">
                    <me>
                        = (3x \times 4x) - (3x \times 3) - (2 \times 4x) + (2 \times 3)
                    </me>
                </p>
                <p xml:id="auto_35h1d2bd">
                    <me>
                        = 12x^2 - 9x - 8x + 6
                    </me>
                </p>
                <p xml:id="auto_o1j1sxjt">
                    <me>
                        = 12x^2 - 17x + 6
                    </me>
                </p>
            </li>
            <li xml:id="auto_yul7nu15">
                <p xml:id="auto_q0t8k8eu">
                    <m>(2x + 3)(3x - 4)</m>
                </p>
                <p xml:id="auto_hasndek4">
                    <me>
                        = (2x \times 3x) - (2x \times 4) + (3 \times 3x) - (3 \times 4)
                    </me>
                </p>
                <p xml:id="auto_hahqlkbf">
                    <me>
                        = 6x^2 - 8x + 9x - 12
                    </me>
                </p>
                <p xml:id="auto_fj9ilkvt">
                    <me>
                        = 6x^2 + x - 12
                    </me>
                </p>
            </li>
        </ol>
    </p>

    <p xml:id="auto_1f64y2z2">
        From the above examples, we can see that the factorisation of a quadratic expression when the coefficient of <m>x^2</m> is not one 
        is similar to the factorisation of a quadratic expression when the coefficient of <m>x^2</m> is one.
    </p>
    <p xml:id="auto_9sooj5fx">
        Factors are multiplied to get the final expresions on the righthand side (RHS) of the equations. 
    </p>

    <investigation xml:id="auto_ima9rin8">
    <p xml:id="auto_y4z9ybzs">
        
    </p>
        <p xml:id="auto_eg3wu936">
            Given the quadratic expressions on the right-hand side of the equation, 
            how can you be able factor them?
        </p>
    </investigation>
    <p xml:id="auto_8gh11y26">
        Consider the expression <m>6x^2 + 7x + 2</m>.
    </p>
    <p xml:id="auto_jmjp6n05">
        The problem can factorised as follows: 
    </p>
    <p xml:id="auto_g4t4y03x">
        <ol xml:id="auto_5ye6huxw" marker="(i)">
            <li xml:id="auto_kipuvx3q">
                <p xml:id="auto_cnkr0wpy">
                    Look for two numbers such that:
                    <ol xml:id="auto_gr4fybpi">
                        <li xml:id="auto_on3h6cew">
                            <p xml:id="auto_jmra5nqg">
                                Their product is equal to the product of the coefficient of <m>x^2</m> and the constant term, i.e. <m>6 \times 2 = 12</m>.
                            </p>
                            <p xml:id="auto_tffzjqb7">
                                In this case <m>6</m> is the coefficient of <m>x^2</m> and <m>2</m> is constant term.
                            </p>
                        </li>
                        <li xml:id="auto_m77fh7su">
                            <p xml:id="auto_t1ubxyzm">
                                Their sum is <m>7</m>, where <m>7</m> is the coefficient of <m>x</m>.
                            </p>
                            <p xml:id="auto_tx41ve8a">
                                The terms are <m>3</m> and <m>4</m>
                            </p>
                        </li>
                    </ol>
                </p>
            </li>
            <li xml:id="auto_bnafdf4g">
                <p xml:id="auto_vfjrbm2n">
                    Rewrite the term <m>7x</m> as the sum of the two numbers found in step <em>(i)(b)</em>.
                </p>
                <p xml:id="auto_34t8qrgh">
                    Thus,
                    <me>
                        6x^2 + 7x + 2 = 6x^2 + 3x + 4x + 2
                    </me>
                </p>
                <p xml:id="auto_thl3e1as">
                    <me>
                        = 3x(2x + 1) + 2(2x + 1)
                    </me>
                </p>
                <p xml:id="auto_kvmoexp9">
                    <me>
                        = (3x + 2)(2x + 1)
                    </me>
                </p>
            </li>
        </ol>
    </p>
    
    <example xml:id="auto_wfijuodu">
        <statement>
            <p xml:id="auto_2x1a4eqn">
                
            </p>
            <p xml:id="auto_ina7w8lj">
                Factorise the expression <m>12x^2 - 17x + 6</m>.
            </p>
        </statement>
        <solution>
            <p xml:id="auto_b7u2e3uw">
                Multiply the coefficient of <m>x^2</m>  (which is 12) by the constant term (which is 6):
                <me>
                    12 \times 6 = 72
                </me>
            </p>
            <p xml:id="auto_3nir9j6e">
                Find two numbers that multiply to give <m>72</m> and add up to <m>-17</m>. The two numbers are <m>-8</m> and <m>-9</m>.
                <me>-9 \times -8 = 72</me> and <me>-9 + -8 = -17</me>
            </p>
            <p xml:id="auto_3kgqbgwt">
                Splt the middle term using these two numbers:
                <me>
                    12x^2 - 9x - 8x + 6
                </me>
            </p>
            <p xml:id="auto_uzzmw2m1">
                Factor by grouping:
                <me>
                    3x(4x - 3) - 2(4x - 3)
                </me>
                Group the factors:
                <me>
                    (3x - 2)(4x - 3)
                </me>                
            </p>

        </solution>
    </example>

    <example xml:id="auto_jyhkd64d">

        <statement>
            <p xml:id="auto_jr8o6ngv">
                
            </p>
            <p xml:id="auto_b3hdywuq">
                Factorise the expression <m>3x^2 - 5x - 2</m>.
            </p>
        </statement>

        <solution>
            <p xml:id="auto_15dsivsq">
                The expression can be factorised as follows:
                <ol xml:id="auto_0w0x7mra">
                    <li xml:id="auto_401etjxc">
                        <p xml:id="auto_scbtuh15">
                            Look for two numbers such that:
                            <ol xml:id="auto_533fpnue">
                                <li xml:id="auto_p6r86bhh">
                                    <p xml:id="auto_4idtvo0t">
                                        Their product is equal to the product of the coefficient of <m>x^2</m> and the constant term, i.e. <m>3 \times -2 = -6</m>.
                                    </p>
                                    <p xml:id="auto_kaxu59ce">
                                        In this case <m>3</m> is the coefficient of <m>x^2</m> and <m>-2</m> is constant term.
                                    </p>
                                </li>
                                <li xml:id="auto_zve4lfzb">
                                    <p xml:id="auto_bk3pz5eb">
                                        Their sum is <m>-5</m>, where <m>-5</m> is the coefficient of <m>x</m>.
                                    </p>
                                    <p xml:id="auto_7kl3zspz">
                                        The terms are <m>-6</m> and <m>1</m>
                                    </p>
                                </li>
                            </ol>
                        </p>
                    </li>
                    <li xml:id="auto_5wfnnbdu">
                        <p xml:id="auto_jws5ajn1">
                            Rewrite the term <m>-5x</m> as the sum of the two numbers found in step 1.
                        </p>
                        <p xml:id="auto_o1d9jw95">
                            Thus,
                            <me>
                                3x^2 - 5x - 2 = 3x^2 - 6x + x - 2
                            </me>
                        </p>
                        <p xml:id="auto_kibonrup">
                            <me>
                                = 3x(x - 2) + 1(x - 2)
                            </me>
                        </p>
                        <p xml:id="auto_fexxksod">
                            <me>
                                = (3x + 1)(x - 2)
                            </me>
                        </p>
                    </li>
                </ol>
            </p>
        </solution>
        
    </example>

    

    <exercises xml:id="exercises-when-the-coefficient-of-x-squared-is-not-one">
        <exercise xml:id="auto_h53xoxuv">
            <statement>
                <p xml:id="auto_wnp3rrtf">
                    Factorise the following expressions:
                    <ol xml:id="auto_vkkg6hnm" marker="1" cols="2">
                        <li xml:id="auto_qniar6m9">
                            <p xml:id="auto_0tlp7him">
                                <ol xml:id="auto_xzvdr8ee" marker="(a)">
                                    <li xml:id="auto_novkkmdx">
                                        <p xml:id="auto_7bf2xgtw">
                                            <m>3x^2 + 4x - 7</m>
                                        </p>
                                    </li>
                                    <li xml:id="auto_7kribh26">
                                        <p xml:id="auto_na1fv7j5">
                                            <m>5x^2 - 9x + 4</m>                                        
                                        </p>
                                    </li>
                                    <li xml:id="auto_std9z736">
                                        <p xml:id="auto_le1v1oci">                                        
                                            <m>11x^2 - 15x + 10</m>                                       
                                        </p>
                                    </li>
                                    <li xml:id="auto_ghc8tzld">
                                        <p xml:id="auto_tpec98ch">                                                                               
                                            <m>17x^2 - 25x + 16</m> 
                                        </p>
                                    </li>
                                </ol>
                            </p>
                        </li>
                        <li xml:id="auto_p2mwxpba">
                            <p xml:id="auto_143peknc">
                                <ol xml:id="auto_idgh14vl" marker="(a)" cols="2">
                                    <li xml:id="auto_63391z0d">
                                        <p xml:id="auto_guxghc2e">
                                            <m>2x^2 + 7x + 3</m>
                                        </p>
                                    </li>
                                    <li xml:id="auto_vq7ycxuv">
                                        <p xml:id="auto_emzbei56">                                        
                                            <m>13x^2 - 17x + 12</m>
                                        </p>
                                    </li>
                                    <li xml:id="auto_t8agorty">
                                        <p xml:id="auto_cci29u9o">                                                                         
                                            <m>6x^2 + 5x - 4</m>
                                        </p>
                                    </li>
                                    <li xml:id="auto_yi7xnmz7">
                                        <p xml:id="auto_5263xvun">                                        
                                            <m>4x^2 + 19x - 13</m>
                                        </p>
                                    </li>
                                </ol>
                            </p>
                        </li>
                        <li xml:id="auto_v7cjo4fk">
                            <p xml:id="auto_5m3oxflh">
                                <ol xml:id="auto_qv2q8du9" marker="(a)" cols="2">
                                    <li xml:id="auto_8d6q9dal">
                                        <p xml:id="auto_6drrxfpm">
                                            <m>7x^2 - 13x + 6</m>
                                        </p>
                                    </li>
                                    <li xml:id="auto_glayrdzr">
                                        <p xml:id="auto_7lga73pe">                                        
                                            <m>8x^2 + 3x - 5</m>
                                        </p>
                                    </li>
                                    <li xml:id="auto_bjy0qc95">
                                        <p xml:id="auto_610ag9xf">                                        
                                            <m>9x^2 - 14x + 8</m>
                                        </p>
                                    </li>
                                    <li xml:id="auto_r8lq7ev7">
                                        <p xml:id="auto_xd2obss6">
                                            <m>10x^2 + 11x - 6</m>
                                        </p>
                                    </li>
                                </ol>
                            </p>
                        </li>
                        <li xml:id="auto_yy6rx1z5">
                            <p xml:id="auto_47pq69wm">
                                <ol xml:id="auto_v6l9s15o" marker="(a)" cols="2">
                                    <li xml:id="auto_u9ccoo6c">
                                        <p xml:id="auto_kstkaqlh">
                                            <m>15x^2 - 21x + 14</m>                                        
                                        </p>
                                    </li>
                                    <li xml:id="auto_2alnz602">
                                        <p xml:id="auto_q7ftnxlr">
                                            <m>4x^2 - 11x + 6</m>
                                        </p>
                                    </li>
                                    <li xml:id="auto_7zs680qk">
                                        <p xml:id="auto_d1xs2aoo">                                        
                                            <m>12x^2 + 13x - 11</m>
                                        </p>
                                    </li>
                                    <li xml:id="auto_vptmp50t">
                                        <p xml:id="auto_a9sxofa3">                                      
                                            <m>16x^2 + 23x - 15</m>                                        
                                        </p>
                                    </li>
                                </ol>
                            </p>
                        </li>
                    </ol>
                </p>
            </statement>
        </exercise>
    </exercises>

</subsubsection>