<stack-static>

    <statement><p>Use the laws of indices to simplify.</p>
<ol class="HELM_parts">
<li><m>x^{10} \times x^{-9}= </m> <fillin characters="7" name="ans1"/>  </li>
<li><m>\dfrac{t^{11}}{t^{-10}}=</m> <fillin characters="7" name="ans2"/>  </li>
<li><m>\dfrac{y^{-5}}{y^{-8}}=</m> <fillin characters="7" name="ans3"/>  </li>
</ol></statement>
    <solution><ol class="HELM_parts">
    <li>Use the first law of indices: </li>
    <p><m>x^{10} \times x^{-9}= x^{{10}+{-9}} =x^{1}= x.</m></p>
    <br>
    <li>Use the second law of indices: </li>
    <p><m>\dfrac{t^{{11}}}{t^{-10}}= t^{{11}-({-10})} = t^{21}.</m></p>
    <br>
    <li>Use the second law of indices, as for (b). <m>\dfrac{y^{{-5}}}{y^{-8}}= y^{{-5}-({-8})} = y^{3}.</m></li>
</ol></solution>
    <answer><p><m>x</m></p></answer>
<answer><p><m>t^{21}</m></p></answer>
<answer><p><m>y^3</m></p></answer>
</stack-static>