<stack-static>
    <statement><div><p>Use the laws of indices to simplify.</p>
<ol class="HELM_parts">
<li><m>\dfrac{a^{9} \times a^{8}}{a^{5}}= </m> <fillin characters="7" name="ans1"/>  </li>
<li><m>\dfrac{m^{10} \times m^{-6}}{m^{-5}}=</m> <fillin characters="7" name="ans2"/>  </li>
</ol></div></statement>
    <solution><ol class="HELM_parts">
    <li>Use the first law of indices to simplify the numerator: </li>
    <p><m>\dfrac{a^{9} \times a^{8}}{a^{5}}= \dfrac{a^{{9}+{8}}}{a^{5}}= \dfrac{a^{{17}}}{a^{5}}.</m></p>
    <p>Now use the second law to simplify the result:</p>
    <p><m>\dfrac{a^{{17}}}{a^{5}}= a^{{17}-{5}} = a^{12}.</m><br/><br/></p>
    <li>Use the first law of indices to simplify the numerator: </li>
    <p><m>\dfrac{m^{10} \times m^{-6}}{m^{-5}}= \dfrac{m^{{10}+{-6}}}{m^{-5}}= \dfrac{m^{{4}}}{m^{-5}}.</m></p>
    <p>Now use the second law to simplify the result:</p>
    <p><m>\dfrac{m^{{4}}}{m^{-5}}= m^{{4}-{-5}} = m^{9}.</m><br/><br/></p>
</ol></solution>
    <answer><p><m>a^{12}</m></p></answer>
    <answer><p><m>m^9</m></p></answer>
</stack-static>