<stack-static>
    <statement><div><p>Consider triangle <m>PQR</m> where <m>\vec{PQ} = \mathbf{u}</m> and <m>\vec{PR} = \mathbf{v}</m>.</p>
<ul>
    <li>Point <m>S</m> is located on <m>PR</m> such that <m>PS : SR = {2} : {4}</m>.</li>
    <li>Point <m>T</m> lies on <m>QR</m> with <m>QT : TR = {1} : {1}</m>.</li>
    <li>Point <m>U</m> is on <m>PQ</m> such that <m>PU : UQ = {2} : {4}</m>.</li>
</ul>

<p>Determine the following vectors in terms of <m>\mathbf{u}</m> and <m>\mathbf{v}</m>.</p>
<p><em>(Enter <m>\mathbf{u}</m> as <c>u</c> and <m>\mathbf{v}</m> as <c>v</c>).</em></p>

<ol class="HELM_parts">
    <li>
        <m>\vec{PS} = </m> <fillin characters="6" name="ans1"/>  
    </li>
    <li>
        <m>\vec{PT} = </m> <fillin characters="6" name="ans2"/>  
    </li>
    <li>
        <m>\vec{PU} = </m> <fillin characters="6" name="ans3"/>  
    </li>
    <li>
        <m>\vec{ST} = </m> <fillin characters="6" name="ans4"/>  
    </li>
    <li>
        <m>\vec{TU} = </m> <fillin characters="6" name="ans5"/>  
    </li>
</ol></div></statement>
    <solution><div><h3>Worked Solution</h3>

<p><alert>(a) Finding <m>\vec{PS}</m></alert></p>
<p>We are given that <m>PS : SR = {2} : {4}</m>. This means the line <m>PR</m> is divided into <m>{2} + {4} = {6}</m> parts.</p>
<p><m>PS</m> represents <m>{2}</m> of those parts.</p>
<me> \vec{PS} = \frac{2}{6}\vec{PR} = \mathbf{\frac{v}{3}} </me>

<p><alert>(c) Finding <m>\vec{PU}</m></alert></p>
<p>Similarly, <m>PU : UQ = {2} : {4}</m>. The line <m>PQ</m> is divided into <m>{2} + {4} = {6}</m> parts.</p>
<me> \vec{PU} = \frac{2}{6}\vec{PQ} = \mathbf{\frac{u}{3}} </me>

<p><alert>(b) Finding <m>\vec{PT}</m></alert></p>
<p>To find <m>\vec{PT}</m>, we first need to travel from <m>P</m> to <m>Q</m>, and then from <m>Q</m> to <m>T</m>: <m>\vec{PT} = \vec{PQ} + \vec{QT}</m>.</p>
<p>First, find <m>\vec{QR}</m>:</p>
<me> \vec{QR} = \vec{PR} - \vec{PQ} = \mathbf{v} - \mathbf{u} </me>
<p>We know <m>QT : TR = {1} : {1}</m>, so <m>QT</m> is <m>\frac{1}{2}</m> of <m>QR</m>.</p>
<me> \vec{QT} = \frac{1}{2}(\mathbf{v} - \mathbf{u}) </me>
<p>Now, add them together:</p>
<me> \vec{PT} = \mathbf{u} + \frac{1}{2}(\mathbf{v} - \mathbf{u}) </me>
<me> \vec{PT} = \mathbf{\frac{v}{2}+\frac{u}{2}} </me>

<p><alert>(d) Finding <m>\vec{ST}</m></alert></p>
<p>Using the triangle rule:</p>
<me> \vec{ST} = \vec{PT} - \vec{PS} </me>
<me> \vec{ST} = \left( {\frac{v}{2}+\frac{u}{2}} \right) - \left( {\frac{v}{3}} \right) </me>
<me> \vec{ST} = \mathbf{\frac{v}{6}+\frac{u}{2}} </me>

<p><alert>(e) Finding <m>\vec{TU}</m></alert></p>
<me> \vec{TU} = \vec{PU} - \vec{PT} </me>
<me> \vec{TU} = \left( {\frac{u}{3}} \right) - \left( {\frac{v}{2}+\frac{u}{2}} \right) </me>
<me> \vec{TU} = \mathbf{-\frac{v}{2}-\frac{u}{6}} </me></div></solution>
    <answer><p><m>\frac{v}{3}</m></p></answer>
    <answer><p><m>\frac{v-u}{2}+u</m></p></answer>
    <answer><p><m>\frac{u}{3}</m></p></answer>
    <answer><p><m>\frac{v-u}{2}-\frac{v}{3}+u</m></p></answer>
    <answer><p><m>-\frac{v-u}{2}-\frac{2 u}{3}</m></p></answer>
</stack-static>