<stack-static>
    <statement><div><p class="HELM_exercise">Exercise</p>
<p>Simplify the following:<br/></p>
<ol class="HELM_parts">
<li><p> <m>{6}\underline{a} + {2}\underline{a} =</m> <fillin characters="5" name="ans1"/>  </p></li>
<li><p> <m>{6}({4}\underline{b}) =</m> <fillin characters="5" name="ans2"/>  </p></li>
<li><p> Expand <m>{4}(\underline{q} + \underline{r}) =</m> <fillin characters="5" name="ans3"/>  </p></li>
</ol>
<p>Write <m>\underline{a}</m> and <m>\underline{b}</m> as <c>a</c> and <c>b</c>, respectively.</p></div></statement>
    <solution><ol class="HELM_parts">
<li><p>The second rule  <m>{6}\underline{a} + {2}\underline{a}</m> can be simplified to <m>{8}\underline{a}.</m></p></li>
<li><p> Using the third rule, <m>{6}({4}\underline{b}) = {24}\underline{b}.</m></p></li>
<li><p> Using the first rule, <m>{4}(\underline{q} + \underline{r}) = {4}\underline{q} + {4}\underline{r}.</m></p></li></ol></solution>
    <answer><p><m>8 a</m></p></answer>
    <answer><p><m>24 b</m></p></answer>
    <answer><p><m>4 r+4 q</m></p></answer>
</stack-static>