<stack-static>
    <statement><div><p>A point <m> M({1}, {1}) </m> undergoes a translation by the vector <m> \begin{pmatrix} {-2} \\ {-5} \end{pmatrix} </m>.</p>
<ol class="HELM_parts">
    <li>
        <p>Determine the coordinates of <m> M' </m>, the transformed point.</p>
       <div><m> M' = </m> <fillin characters="7" name="ans1"/> </div>
    </li>
    <li>
        <p>If <m> M' </m> is then translated by <m> \begin{pmatrix} {-5} \\ {6} \end{pmatrix} </m>, find the final position <m> M'' </m>.</p>
        <div><m> M'' = </m> <fillin characters="7" name="ans2"/> </div>
    </li>
    <li>
        <p>What is the single translation vector that maps <m> M </m> to <m> M'' </m> directly?</p>
        <div>Vector = <fillin characters="7" name="ans3"/> </div>
    </li>
</ol>
<p> </p></div></statement>
    <solution><div><h3>Worked Solution</h3>

<p><alert>Part (a): Finding M'</alert></p>
<p>To translate a point <m>M(x, y)</m> by a vector <m>\begin{pmatrix} a \\ b \end{pmatrix}</m>, we add the vector components to the point's coordinates:</p>
<me> M' = \begin{pmatrix} {1} \\ {1} \end{pmatrix} + \begin{pmatrix} {-2} \\ {-5} \end{pmatrix} = \begin{pmatrix} {1} + {-2} \\ {1} + {-5} \end{pmatrix} = \begin{pmatrix} {-1} \\ {-4} \end{pmatrix} </me>
<p>So, the coordinates of <m> M' </m> are <m> ({-1}, {-4}) </m>.</p>

<p><alert>Part (b): Finding M''</alert></p>
<p>Now we translate <m> M' </m> by the second vector <m>\begin{pmatrix} {-5} \\ {6} \end{pmatrix}</m>:</p>
<me> M'' = \begin{pmatrix} {-1} \\ {-4} \end{pmatrix} + \begin{pmatrix} {-5} \\ {6} \end{pmatrix} = \begin{pmatrix} {-1} + {-5} \\ {-4} + {6} \end{pmatrix} = \begin{pmatrix} {-6} \\ {2} \end{pmatrix} </me>
<p>The final position is <m> M''({-6}, {2}) </m>.</p>

<p><alert>Part (c): Single Translation Vector</alert></p>
<p>The single translation vector that maps the start <m>M</m> directly to the end <m>M''</m> is the sum of the two individual translation vectors:</p>
<me> \mathbf{v}_{total} = \mathbf{v}_1 + \mathbf{v}_2 </me>
<me> \mathbf{v}_{total} = \begin{pmatrix} {-2} \\ {-5} \end{pmatrix} + \begin{pmatrix} {-5} \\ {6} \end{pmatrix} = \begin{pmatrix} {-2} + {-5} \\ {-5} + {6} \end{pmatrix} = \begin{pmatrix} {-7} \\ {1} \end{pmatrix} </me>
<p>Alternatively, you can subtract the starting point from the end point:</p>
<me> M'' - M = \begin{pmatrix} {-6} \\ {2} \end{pmatrix} - \begin{pmatrix} {1} \\ {1} \end{pmatrix} = \begin{pmatrix} {-7} \\ {1} \end{pmatrix} </me></div></solution>
    <answer><p><m>\left[\begin{array}{c} -1 \\ -4 \end{array}\right]</m></p></answer>
    <answer><p><m>\left[\begin{array}{c} -6 \\ 2 \end{array}\right]</m></p></answer>
    <answer><p><m>\left[\begin{array}{c} -7 \\ 1 \end{array}\right]</m></p></answer>
</stack-static>