<subsubsection xml:id="subsubsec-perfect-squares" xmlns:xi="http://www.w3.org/2001/XInclude">
    <title>Perfect Squares</title>

    <activity xml:id="auto_upsvqrlr">
        <p xml:id="auto_60id38ad">
            <em><term>Work in Groups.</term></em>
        </p>
        <p xml:id="auto_em4y8k0p"> 
            Define, discuss, and work on the following:
            <ol xml:id="auto_dgezk56f">
                <li xml:id="auto_mgzczpef">
                    <p xml:id="auto_mqwqnjpz">Perfect square identities.</p>
                </li>
                <li xml:id="auto_hwnj4hbm">
                    <p xml:id="auto_9syzqcw1">Expanding perfect squares.</p>
                </li>
                <li xml:id="auto_1tw9p6yi">
                    <p xml:id="auto_pcfz65rz">Recognizing perfect square trinomials.</p>
                </li>
                <li xml:id="auto_0svm5l5y">
                    <p xml:id="auto_tzvjzwik">Factoring perfect square trinomials.</p>
                </li>
            </ol>
        </p>
        <p xml:id="auto_nkrnfucs">
            Copy the following expressions and identities, observe and discuss:
            <ol xml:id="auto_tp8bziyo" marker="(i).">
                <li xml:id="auto_ttzs6lar">
                    <p xml:id="auto_262rt19n"><m>(a + b)^2 = a^2 + 2ab + b^2</m></p>
                </li>
                <li xml:id="auto_5weqiq82">
                    <p xml:id="auto_8r6cwqa4"><m>(a - b)^2 = a^2 - 2ab + b^2</m></p>
                </li>  
            </ol>
            Recognize the middle term is twice the product of the two terms.
        </p>
        <p xml:id="auto_f8uc5rg9">
            <ul xml:id="auto_mo3g0h30">
                <li xml:id="auto_wthrqp5d">
                    <p xml:id="auto_k8pxsriy">Compare the different approaches groups used to solve similar problems.</p>
                </li>
                <li xml:id="auto_5ydy2v64">
                    <p xml:id="auto_f8zlotpo">Discuss how perfect square identities can make simplification and factoring easier.</p>
                </li>
                <li xml:id="auto_mvf3ns9k">
                    <p xml:id="auto_lqjh1gym">Explore how these identities are useful in different contexts (e.g., solving quadratic equations, simplifying expressions in algebra).</p>
                </li>
                <li xml:id="auto_u4kupvzf">
                    <p xml:id="auto_oaojf0ju">How do perfect square identities help us solve quadratic expressions faster?</p>
                </li>
                <li xml:id="auto_xt1kl7jq">
                    <p xml:id="auto_c8qtmt5t">What happens if we don't recognize the identity right awayâ€”how might that slow us down?</p>
                </li>
                <li xml:id="auto_nmx814fp">
                    <p xml:id="auto_kas1zw74">Can you think of any real-world applications where you might use perfect square identities?</p>
                </li>
            </ul>
        </p>
    </activity>

    <p xml:id="auto_ph5a57bb">
        A <em><term>Perfect Square</term></em> is a special kind of trinomial that can be factored into the square of a binomial. 
        There are two forms of perfect square identities:
    </p>
    <ul>
        <li xml:id="auto_qzb0huct">
            <p xml:id="auto_c7tomgv2">
                <m> (a + b)^2 = a^2 + 2ab +b^2  </m>, and
            </p>
        </li>
        <li xml:id="auto_5jggf73c">
            <p xml:id="auto_aa7dae8a">
                <m> (a - b)^2 = a^2 - 2ab +b^2  </m>
            </p>
        </li>
    </ul>
    
    <p xml:id="auto_i4t6pl2v">
        In these identities, the expression on the left is a perfect square, which means it can be written as the square of a binomial (a two-term expression). 
        The first identity is used when the middle term is positive, and the second identity is used when the middle term is negative.
    </p>

    <example xml:id="auto_zyorrwjd">
    <title>(Using the first identity)</title>
        
        <statement>
            <p xml:id="auto_zpcpym79">
                
            </p>
            <p xml:id="auto_tvnempk9">
                Consider the quadratic below:
                <me>
                    x^2 + 6x + 9
                </me>                    
            </p>
        </statement>

        <solution>
            <p xml:id="auto_0ts8xawo">
                The expression <m>x^2 + 6x + 9</m> is perfefect square. A perfect square follows the pattern:
                <md>
                    <mrow> (a + b)^2 \amp = a^2 + 2ab + b^2 </mrow>
                </md>
            </p>
            <p xml:id="auto_td33sff2">
                Here, <m>a^2 = x^2, 2ab = 6x</m> and <m>b^2 = 9.</m> The square roots of <m>x^2</m> and <m>9</m> are <m>x</m> and <m>3,</m>
                respectively.
            </p>
            <p xml:id="auto_sw9gtqa8">
                In this case, the expression <m>x^2 + 6x + 9</m> matches the form <m>a^2 + 2ab + b^2,</m> where:
                <ul xml:id="auto_ifqv4bkt">
                    <li xml:id="auto_k9syx8w3">
                        <p xml:id="auto_dffzxwkt">
                            <m>a = x,</m>
                        </p>
                    </li>
                    <li xml:id="auto_qowjr8n3">
                        <p xml:id="auto_kv23941k">
                            <m>b = 3.</m>
                        </p>
                    </li>
                </ul>
            </p>
            <p xml:id="auto_3irp63l0">
                The middle term <m>2ab</m> is <m>6x,</m> which fits the formula for a perfect square with a negative middle term. 
                Applying the identity:
                <md>
                <mrow>x^2 + 6x + 9 \amp = (x + 3)^2 </mrow>
                </md>
                So, <m>x^2 + 6x + 9</m> factors into <m>(x + 3)^2.</m>
            </p>
        </solution>

    </example>

    <example xml:id="auto_0u8ldn3b">
    <title>(Using the second identity)</title>

        <statement>
            <p xml:id="auto_5oh4x0jc">
                
            </p>
            <p xml:id="auto_vcdf68tz">
                Using the quadratic below:
                <me>
                    x^2 - 10x + 25
                </me>                    
            </p>
        </statement>

        <solution>
            <p xml:id="auto_7lpgaony">
                The expression <m>x^2 - 10x + 25</m> matches the form <m>a^2 - 2ab + b^2</m> where:
                <ul xml:id="auto_syrx4qe4">
                    <li xml:id="auto_8kzgheo0">
                        <p xml:id="auto_gzy5i5jd">
                            <m>a = x,</m>
                        </p>
                    </li>
                    <li xml:id="auto_nj36ro7f">
                        <p xml:id="auto_05loeg22">
                            <m>b = 5.</m>
                        </p>
                    </li>
                    <li xml:id="auto_p77rwm56">
                        <p xml:id="auto_i22knxqa">
                            The middle term <m>2ab = -10x,</m> and the constant term <m>b^2 = 25.</m>
                        </p>
                    </li>
                </ul>
            </p>
            <p xml:id="auto_3w6x84oc">
                So, this is a perfect square, and we can factor it as:
                <md>
                    <mrow>x^2 - 10x + 25 \amp = (x - 5)^2 </mrow>
                </md>
            </p>
        </solution>

    </example>

</subsubsection>