<subsubsection xml:id="subsubsec-difference-of-squares" xmlns:xi="http://www.w3.org/2001/XInclude">
<title>Difference of Squares</title>

        <activity xml:id="auto_5vdy1rrm">
            <p xml:id="auto_kebikz01">
                <em><term>Work in Groups.</term></em>
            </p>
            <p xml:id="auto_1mrno69e"> 
                Define, discuss, and work on the following:
                <ol xml:id="auto_i379lbk0">
                    <li xml:id="auto_lqve6ykm">
                        <p xml:id="auto_llg5ih49">Difference of squares.</p>
                    </li>
                    <li xml:id="auto_czemvt39">
                        <p xml:id="auto_lujm8txv">Identifying difference of squares in algebraic expressions.</p>
                    </li>
                    <li xml:id="auto_uk32351i">
                        <p xml:id="auto_h3bfiafz">Factoring using the difference of squares formula.</p>
                    </li>
                    <li xml:id="auto_nuhp8p38">
                        <p xml:id="auto_pjoniwco">Recognizing patterns when applying the difference of squares.</p>
                    </li>
                </ol>
            </p>
            <p xml:id="auto_4e0lyyn2">
                Copy the following expressions and identities, observe and discuss:
                <ol xml:id="auto_88v1oqz5" marker="(i).">
                    <li xml:id="auto_kbd0mldo">
                        <p xml:id="auto_uk8y0qot"><m>a^2 - b^2 = (a + b)(a - b)</m> (Difference of squares)</p>
                    </li>
                </ol>
                Recognize how the difference of squares applies to algebraic expressions.
            </p>
            <p xml:id="auto_zgaissvf">
                <ul xml:id="auto_m17qd3wf">
                    <li xml:id="auto_m1fl46ex">
                        <p xml:id="auto_rni9c2jn">Compare the different approaches groups used to solve similar problems.</p>
                    </li>
                    <li xml:id="auto_3tthjgxw">
                        <p xml:id="auto_ivgjdyg8">Discuss how the difference of squares formula makes factoring easier.</p>
                    </li>
                    <li xml:id="auto_4sy3smni">
                        <p xml:id="auto_ajq59jry">Explore how this identity is useful in different contexts (e.g., simplifying expressions, solving equations).</p>
                    </li>
                    <li xml:id="auto_mcj9d9xa">
                        <p xml:id="auto_t9oof3oj">How does recognizing the difference of squares help in solving quadratic equations?</p>
                    </li>
                    <li xml:id="auto_nx2pl1z1">
                        <p xml:id="auto_zrezfkos">What happens if we don't recognize the difference of squaresâ€”how might that affect solving the problem?</p>
                    </li>
                    <li xml:id="auto_ueblvvmz">
                        <p xml:id="auto_q55lyids">Can you think of any real-world applications where the difference of squares might be used?</p>
                    </li>
                </ul>
            </p>
        </activity>

        <p xml:id="auto_hrjwzemb">
            The <em><term>Difference of Squares</term></em> is an identity that applies when you have two terms that are perfect squares and are being subtracted from each other. 
            The identity states:
            <md>
                <mrow>a^2 - b^2 \amp = (a - b)(a + b) </mrow>
            </md>
            This means that the difference between two squares can be factored into the product of two binomials: 
            one where the terms are subtracted and one where the terms are added.
        </p>

        <p xml:id="auto_b6uq15a2">
            In the expression <m>a^2 - b^2</m>, <m>a</m> and <m>b</m> represent the square roots of the two terms. 
            When you subtract two perfect squares, you can factor the expression as the product of two binomials: 
            <m>(a - b)</m> and <m>(a + b)</m>.
        </p>

        <example xml:id="auto_uz3zuoi4">
            <statement>
                <p xml:id="auto_n99ayvze">
                    
                </p>
                <p xml:id="auto_mwgh5b81">
                    Consider the quadratic, solve:
                    <md>
                        <mrow> \amp x^2 - 16</mrow>
                    </md>
                </p>
            </statement>
            <solution>
                <p xml:id="auto_o1p0237v">
                    The expression <m>x^2 - 16</m> is in the form of a difference of squares, which follows the identity:
                    <md>
                        <mrow>a^2 - b^2 \amp = (a -b)(a + b) </mrow>
                    </md>
                </p>
                <p xml:id="auto_fcq8mc8m">
                    In this case, <m>a^2 = x^2</m> and <m>b^2 = 16.</m> The square roots of <m>x^2</m> and <m>16</m> are <m>x</m> and <m>4,</m>
                    respectively.
                    We can rewrite the expression as:
                    <md>
                        <mrow> x^2 - 16 \amp = x^2 - 4^2 </mrow>
                    </md>
                    Applying the difference of squares identity we have:
                    <md>
                        <mrow>x^2 - 16 \amp = (x - 4)(x + 4) </mrow>
                    </md>
                </p>
            </solution>
        </example>

    </subsubsection>