<subsection xml:id="subsec-quadratic-identities" xmlns:xi="http://www.w3.org/2001/XInclude">
    <title>Quadratic Identities</title>

    <introduction xml:id="auto_2c5i50a8">
        <axiom component="resources">
        <!-- Link to blurb -->
        <xi:include href="../../resources-blurb-subsec.ptx" />

        <sbsgroup widths="45% 45%" margins="2% 2%">
            <sidebyside>
                <p xml:id="auto_c5x6yajh">
                    My learners <alert>do not have access</alert> to devices during class:                  
                </p>
                <p xml:id="auto_cdg9ezec">
                    My learners <alert>have access</alert> to devices during class:
                </p>
            </sidebyside>        
            <sidebyside>
                <p xml:id="auto_e2ve6iul">
                    <dataurl source="lesson-plans/Numbers and Algebra/Quadratics Expressions and Equations 1/Without Devices PDFs/Quadratic Identities.pdf"> Offline lesson plan </dataurl>
                </p>
                <p xml:id="auto_mci3ajmg">
                    <dataurl source="lesson-plans/Numbers and Algebra/Quadratics Expressions and Equations 1/With Devices PDFs/Quadratic Identities.pdf"> Online lesson plan</dataurl>
                </p>
            </sidebyside>
            <sidebyside>
                <p xml:id="auto_o8u9iygy">
                    <dataurl source="lesson-plans/Numbers and Algebra/Quadratics Expressions and Equations 1/Without Devices PDFs/Step by step guide_Quadratic Identities.pdf"> Offline step-by-step guide</dataurl>
                </p>
                <p xml:id="auto_1fqfmbtu">
                    <dataurl source="lesson-plans/Numbers and Algebra/Quadratics Expressions and Equations 1/With Devices PDFs/Step by step guide_Quadratic Identities.pdf"> Online step-by-step guide</dataurl>
                </p>
            </sidebyside>
        </sbsgroup>
    </axiom>
            <p>
                In algebra, an <term>identity</term> is an equation that is true for all values of the variable.
            </p>

            <p>
                A <term>quadratic identity</term> is an identity in which the highest power of the variable is <m>2</m>.
            </p>

            <p>
                For example:
                <m>(x+1)^2 = x^2 + 2x + 1</m>
            </p>

            <p>
                Both sides contain the variable <m>x</m>, and both sides give the same result for any value of <m>x</m>. 
                Therefore, this equation is an identity.
            </p>

            <p>
                In this section, we will learn some important quadratic identities that help us expand and factorise algebraic expressions.
            </p>
            <p>
                <ul>
                    <li>Perfect Square identities</li>
                    <li>Difference of Squares identities</li>
                </ul>
            </p>
            <note>
                <p>
                    Important quadratic identities are useful because they make algebraic calculations faster and easier. 
                    You should learn the main ones and practise using them.
                </p>
            </note>
    </introduction>

    <xi:include href="subsubsec-perfect-squares.ptx" />

    <xi:include href="subsubsec-difference-of-squares.ptx" />

    <xi:include href="subsubsec-quadratic-identities-in-numerical-cases.ptx" />
    
    <exercises xml:id="exercises-quadratic-identites">
        <exercise xml:id="auto_vrpu3mpz">
        <statement>
            <p xml:id="auto_x97r462m">
                Use the quadratic identities to write down the expansions of each of the following expressions:
                <ol xml:id="auto_sxpul0nj" cols="2">
                    <li xml:id="auto_7zynfoh0">
                        <p xml:id="auto_h99i5n6o">
                            <m>(4x + 5)^2</m>
                        </p>
                    </li>
                    <li xml:id="auto_2fv0gydm">
                        <p xml:id="auto_slsqgaem">
                            <m>\left( \frac{1}{x} + \frac{1}{y} \right) \left( \frac{1}{x} - \frac{1}{y} \right)</m>
                        </p>
                    </li>
                    <li xml:id="auto_i03wxlwm">
                        <p xml:id="auto_hbnit651">
                            <m>(8 - x)^2</m>
                        </p>
                    </li>
                    <li xml:id="auto_za1ax27l">
                        <p xml:id="auto_nhy11zcc">
                            <m>(x - 7)^2</m>
                        </p>
                    </li>
                    <li xml:id="auto_4azwnpk5">
                        <p xml:id="auto_zqr748n4">
                            <m>\left( x + \frac{1}{2} \right)^2</m>
                        </p>
                    </li>
                    <li xml:id="auto_i1enkgdp">
                        <p xml:id="auto_79bagkb7">
                            <m>\left( \frac{1}{4} - \frac{3}{4}b \right)^2</m>
                        </p>
                    </li>
                    <li xml:id="auto_t711fpen">
                        <p xml:id="auto_b43x95ov">
                            <m>(x + 2)^2</m>
                        </p>
                    </li>
                    <li xml:id="auto_e6g40ep4">
                        <p xml:id="auto_drkv8zli">
                            <m>(x + 5)^2</m>
                        </p>
                    </li>
                </ol>
            </p>
        </statement>
        <answer>
            <p xml:id="auto_t85p89sy">
                <ol marker="(a)">
                    <li xml:id="auto_gajcnhhm">
                        <p xml:id="auto_8rrgn3fg">
                            Using the perfect squares identity:
                            <md>
                                <mrow>(4x + 5)^2 \amp = (4x)^2 + 2(4x)(5) + 5^2</mrow>
                                <mrow>\amp = 16x^2 + 40x + 25</mrow>
                            </md>
                        </p>
                    </li>
                    <li xml:id="auto_q47qipbw">
                        <p xml:id="auto_zgclfnds">
                            Using the difference of squares identity:
                            <md>
                                <mrow>\left( \frac{1}{x} + \frac{1}{y} \right) \left( \frac{1}{x} - \frac{1}{y} \right) \amp = \left( \frac{1}{x} \right)^2 - \left( \frac{1}{y} \right)^2</mrow>
                                <mrow>\amp = \frac{1}{x^2} - \frac{1}{y^2}</mrow>
                            </md>
                        </p>
                    </li>
                    <li xml:id="auto_7dokup6b">
                        <p xml:id="auto_yq6oq8rt">
                            Using the perfect squares identity:
                            <md>
                                <mrow>(8 - x)^2 \amp = 8^2 - 2(8)(x) + x^2</mrow>
                                <mrow>\amp = x^2 - 16x + 64</mrow>
                            </md>
                        </p>
                    </li>
                    <li xml:id="auto_63sczc0g">
                        <p xml:id="auto_rmx52f5k">
                            Using the perfect squares identity:
                            <md>
                                <mrow>(x - 7)^2 \amp = x^2 - 2(x)(7) + 7^2</mrow>
                                <mrow>\amp = x^2 - 14x + 49</mrow>
                            </md>
                        </p>
                    </li>
                    <li xml:id="auto_lb42zhm3">
                        <p xml:id="auto_9lavlcgk">
                            Using the perfect squares identity:
                            <md>
                                <mrow>\left( x + \frac{1}{2} \right)^2 \amp = x^2 + 2\left(x\right)\left(\frac{1}{2}\right) + \left(\frac{1}{2}\right)^2</mrow>
                                <mrow>\amp = x^2 + x + \frac{1}{4}</mrow>
                            </md>
                        </p>
                    </li>
                    <li xml:id="auto_sldtts4z">
                        <p xml:id="auto_e8qwrx49">
                            Using the perfect squares identity:
                            <md>
                                <mrow>\left( \frac{1}{4} - \frac{3}{4}b \right)^2 \amp = \left( \frac{1}{4} \right)^2 - 2\left( \frac{1}{4} \right)\left( \frac{3}{4}b \right) + \left( \frac{3}{4}b \right)^2</mrow>
                                <mrow>\amp = \frac{1}{16} - \frac{3}{8}b + \frac{9}{16}b^2</mrow>
                            </md>
                        </p>
                    </li>
                    <li xml:id="auto_oqv9859m">
                        <p xml:id="auto_as6gwvx1">
                            Using the perfect squares identity:
                            <md>
                                <mrow>(x + 2)^2 \amp = x^2 + 2(x)(2) + 2^2</mrow>
                                <mrow>\amp = x^2 + 4x + 4</mrow>
                            </md>
                        </p>
                    </li>
                    <li xml:id="auto_nvhrz05i">
                        <p xml:id="auto_ncmceo8q">
                            Using the perfect squares identity:
                            <md>
                                <mrow>(x + 5)^2 \amp = x^2 + 2(x)(5) + 5^2</mrow>
                                <mrow>\amp = x^2 + 10x + 25</mrow>
                            </md>
                        </p>
                    </li>
                </ol>
            </p>
        </answer>
        </exercise>
    </exercises>

</subsection>