<subsubsection xml:id="subsubsec-factorising-monic-quadratics" xmlns:xi="http://www.w3.org/2001/XInclude">
    <title>Factorising Monic Quadratics</title>
    <objectives component="outcomes">
        <introduction>
            <dl>
                <li>
                    <title>Strand</title>
                    <p>
                        1.0 Numbers and Algebra
                    </p>
                </li>
                <li>
                    <title>Sub-Strand</title>
                    <p>
                        1.3 Quadratic Expressions and Equations
                    </p>
                </li>
            </dl>
        </introduction>
        <ul>
            <li>Factorise quadratic expressions from different situations</li>
        </ul>
    </objectives>
        <axiom component="resources">
        <!-- Link to blurb -->
        <xi:include href="../../resources-blurb-lesson.ptx" />

        <sbsgroup widths="45% 45%" margins="2% 2%">
            <sidebyside>
                <p>
                    <dataurl source="lesson_plans/numbers-and-algebra/quadratic-expressions-and-equations/factorising-monic-quadratics.pdf"> Lesson Plan </dataurl>
                </p>
                <p>
                    <dataurl source="lesson_plans/numbers-and-algebra/quadratic-expressions-and-equations/step-by-step-guide_factorising-monic-quadratics.pdf"> Step-by-Step Guide </dataurl>
                </p>
            </sidebyside>
        </sbsgroup>
    </axiom>


    <p xml:id="auto_dp73d5r0">
        The expression
        <me>
            ax^2 + bx + c,
        </me>
        where <m>a, b, c</m> are constants and <m>a \neq 0</m>, is called a quadratic expression.
    </p>
    <p xml:id="auto_eyjfk2xh">
        In such expressions <m>a</m> is called the coefficient of <m>x^2</m>, <m>b</m> is called the coefficient of <m>x</m> and <m>c</m> is called the constant term.
    </p>
    <p xml:id="auto_kmekc0hk">
        When the coefficient of <m>x^2</m> is one, the expression is of the form;
        <me>
            x^2 + bx + c.
        </me>
    </p>
    <p xml:id="auto_hvjoe6cl">
        Cosider the following expressions:
        
    </p>
    <sidebyside>
    <p xml:id="auto_k6zseta3">
        <me>
            \text{(a).} \, (x + 3)(x + 4).
        </me>
    </p>
    <p xml:id="auto_26ypz13r">            
        <me>
           \text{(b).} \, (x -6)(x - 5).
        </me>                
    </p>
    </sidebyside>
    <sidebyside>
        <p xml:id="auto_ja7aehx1">
            Expanding the expressions we get:               
            <md>
                <mrow>(x + 3)(x + 4) \amp = x(x + 3) + 4(x + 3) </mrow>
            </md>
            <md>
                <mrow>(x + 3)(x + 4) \amp = x^2 + 3x + 4x + 12 </mrow>
            </md>
            Collecting like terms to get:
            <me>
                x^2 + 7x + 12.
            </me>
        </p>
        <p xml:id="auto_5lpsd36p">
            <m>\,</m>
        </p>
    <p xml:id="auto_xdse0lpa">
        Expanding the expressions we get:
        <md>
            <mrow>(x - 6)(x - 5) \amp = x(x - 5) - 6(x - 5) </mrow>
        </md>
        <md>
            <mrow>(x - 6)(x - 5) \amp = x^2 - 5x - 6x + 30 </mrow>
        </md>
        Simplify the middle terms:
        <me>
            x^2 - 11x + 30.
        </me>
    </p>
    </sidebyside>
    
    <p xml:id="auto_cn640cin">
        From the above examples, we can see that the expressions <m>x^2 + 7x + 12</m> and <m>x^2 - 11x + 30</m> are formed from the factors of expressions <m>(x + 3)(x + 4)</m> and <m>(x - 6)(x - 5)</m> respectively.
    </p>
    <p xml:id="auto_bge1pybj">
        The factorised form of the expression <m>x^2 + bx + c</m> is <m>(x + m)(x + n)</m> where <m>m</m> and <m>n</m> are the factors of <m>c</m> whose sum is <m>b</m>.
    </p>
    <p xml:id="auto_rvpg68qv">
        In each case;
        <ol xml:id="auto_qbepzv8i" marker="i">
            <li xml:id="auto_ug26ym22">
                <p xml:id="auto_0rkvaefj">
                    The sum of the constant terms in the factors is equal to the coefficient of <m>x</m> in the expression.
                </p>
            </li>
            <li xml:id="auto_fwl91cd1">
                <p xml:id="auto_7bow7r0y">
                    The product of the constant terms in the factors is equal to the constant term in the expression.
                </p>
            </li>
        </ol>
    </p>

    <example xml:id="auto_yrl3h9s0">
        <statement>
            <p xml:id="auto_mgkno0sg">
                
            </p>
            <p xml:id="auto_wssgp0pk">
                Factorise the following expression:
                <me>
                    x^2 + 5x + 6.
                </me>
            </p>
        </statement>
        <solution>
            <p xml:id="auto_ayw868ip">
                In this case, the coefficient of <m>x^2</m> is one, the coefficient of <m>x</m> is 5 and the constant term is 6.
            </p>
            <p xml:id="auto_ufbderfr">
                So the factors will be of the form <m>(x + m)(x + n)</m> where <m>m</m> and <m>n</m> are the factors of 6 whose sum is 5.
            </p>
            <p xml:id="auto_9rzvlze2">
                In the expression <m>x^2 + 5x + 6</m>, look for two numbers such the numbers <m>a</m> and <m>b</m> such that 
                <me>a + b = 5</me> is coefficient of <m>x</m> and <m>ab = 6</m> is the constant term.
            </p>
            <p xml:id="auto_33r4n2vz">
                In this case, the numbers are 2 and 3.
            </p>
            <p xml:id="auto_bojq5qrm">
                <me>
                    x^2 + 5x + 6 = x^2 + 2x + 3x + 6.
                </me>                
            </p>
            <p xml:id="auto_7r8scwv4">
                Grouping terms, we get:
            </p>
            <p xml:id="auto_w08tg6un">
                <me>
                    x^2 + 5x + 6 = x(x + 2) + 3(x + 2). <!-- Grouping terms -->
                </me>
            </p>
            <p xml:id="auto_j4jtwh8a">
                <me>
                    x^2 + 5x + 6 = (x + 2)(x + 3).
                </me>
            </p>
            <p xml:id="auto_294mn8zi">
                Therefore, the factorised form of the expression <m>x^2 + 5x + 6</m> is <m>(x + 2)(x + 3)</m>.
            </p>
        </solution>
    </example>

    <example xml:id="auto_y55gwt1n">
        <statement>
            <p xml:id="auto_lfloruyg">
                
            </p>
            <p xml:id="auto_g8ypuoew">
                Factorise the following expression:
                <me>
                    x^2 - 9x + 20.
                </me>
            </p>
        </statement>
        <solution>
            <p xml:id="auto_3r83c8me">
                Look for two numbers such that the numbers <m>a</m> and <m>b</m> such that <m>a + b = -9</m> and <m>ab = 20</m>.
            </p>
            <p xml:id="auto_3rl3xhl7">
                The numbers are -4 and -5.
            </p>
            <p xml:id="auto_0s2trovc">
                Then, the expression <m>x^2 - 9x + 20</m> can be written as:
                <me>
                    x^2 - 4x - 5x + 20.
                </me>                
            </p>
            <p xml:id="auto_ht8kos7u">
                Grouping terms, we get:
                <me>
                    x^2 - 9x + 20 = x(x - 4) - 5(x - 4).
                </me>                
            </p>
            <p xml:id="auto_ld1heie0">
                <me>
                    x^2 - 9x + 20 = (x - 4)(x - 5).
                </me>
            </p>
            <p xml:id="auto_hdkv36vm">
                The factorised form of the expression <m>x^2 - 9x + 20</m> is <m>(x - 4)(x - 5)</m>.
            </p>
        </solution>
    </example>

    <example xml:id="auto_7vmdrnv7">
        <statement>
            <p xml:id="auto_wsgwtp0e">
                
            </p>
            <p xml:id="auto_u8y3zind">
                Factorise the following expression:
                <me>
                    x^2 + 6x + 9.
                </me>
            </p>
        </statement>
        <solution>
            <p xml:id="auto_o0jum3kk">
                Look for two numbers such that the numbers <m>a</m> and <m>b</m> such that <m>a + b = 6</m> and <m>ab = 9</m>.
            </p>
            <p xml:id="auto_hrptcxzo">
                The numbers are 3 and 3.
            </p>
            <p xml:id="auto_cuz5fk9t">
                Then, the expression <m>x^2 + 6x + 9</m> can be written as:
                <me>
                    x^2 + 3x + 3x + 9.
                </me>
            </p>
            <p xml:id="auto_zygep1u9">
                Grouping terms, we get:
                <me>
                    x^2 + 6x + 9 = x(x + 3) + 3(x + 3).
                </me>
            </p>
            <p xml:id="auto_vxv0bqrv">
                <me>
                    x^2 + 6x + 9 = (x + 3)(x + 3).
                </me>
            </p>
            <p xml:id="auto_wk4dgwqp">
                The factorised form of the expression <m>x^2 + 6x + 9</m> is <m>(x + 3)(x + 3)</m>.
            </p>
        </solution>
    </example>

    <exercises xml:id="exercises-when-cofficient-of-x-squared-is-one">
        <exercise xml:id="auto_efnrotnf">
            <statement>
                <p xml:id="auto_uug3fpeh">
                    Factorise the following expressions:
                    <ol xml:id="auto_qb9ysrlw" marker="(a)." cols="3">
                        <li xml:id="auto_lak6jvxn">
                            <p xml:id="auto_vn5sovja">
                                <m>
                                    x^2 + 4x + 4.
                                </m>
                            </p>
                        </li>
                        <li xml:id="auto_cv4lswko">
                            <p xml:id="auto_pzlunqie">
                                <m>
                                    x^2 + 8x + 15.
                                </m>
                            </p>
                        </li>
                        <li xml:id="auto_2vmawb3e">
                            <p xml:id="auto_ldm0dfev">
                                <m>
                                    x^2 - 7x + 12.
                                </m>
                            </p>
                        </li>
                        <li xml:id="auto_qtlv2j9s">
                            <p xml:id="auto_b4u3ihm6">
                                <m>
                                    x^2 - 6x + 9.
                                </m>
                            </p>
                        </li>
                        <li xml:id="auto_01e4b0w2">
                            <p xml:id="auto_l6vv8u4z">
                                <m>
                                    x^2 + 3x + 2.
                                </m>
                            </p>
                        </li>
                        <li xml:id="auto_cr7a2xnb">
                            <p xml:id="auto_dajblsdz">
                                <m>
                                    x^2 - 5x + 6.
                                </m>
                            </p>
                        </li>
                        <li xml:id="auto_u91khnzo">
                            <p xml:id="auto_2edn7rz0">
                                <m>
                                    x^2 + 2x - 15.
                                </m>
                            </p>
                        </li>
                        <li xml:id="auto_s4838u0g">
                            <p xml:id="auto_aq8rkm9j">
                                <m>
                                    x^2 - 4x - 5.
                                </m>
                            </p>
                        </li>
                        <li xml:id="auto_zwl1kdbu">
                            <p xml:id="auto_lzlwybni">
                                <m>
                                    x^2 - 3x - 10.
                                </m>
                            </p>
                        </li>
                        <li xml:id="auto_ps0n5siv">
                            <p xml:id="auto_2abvrknj">
                                <m>
                                    x^2 + 7x + 10.
                                </m>
                            </p>
                        </li>
                        <li xml:id="auto_arqnj7z1">
                            <p xml:id="auto_6d1azi6c">
                                <m>
                                    x^2 - 8x - 20.
                                </m>
                            </p>
                        </li>
                        <li xml:id="auto_bwn7cjw6">
                            <p xml:id="auto_z96jygir">
                                <m>
                                    x^2 + 9x + 20.
                                </m>
                            </p>
                        </li>
                    </ol>
                </p>
            </statement>
            <answer>
                <p xml:id="auto_w29rfqcf">
                    <ol marker="(a).">
                        <li xml:id="auto_lp3za9wr">
                            <p xml:id="auto_2zcjrll6">
                                We need two numbers that add to <m>4</m> and multiply to <m>4</m>; <m>2</m> and <m>2</m> work, so separate the middle term:
                                <md>
                                    <mrow>x^2 + 4x + 4 \amp = x^2 + 2x + 2x + 4</mrow>
                                    <mrow>\amp = x(x + 2) + 2(x + 2)</mrow>
                                    <mrow>\amp = (x + 2)(x + 2)</mrow>
                                </md>
                            </p>
                        </li>
                        <li xml:id="auto_mokqr8mf">
                            <p xml:id="auto_0k1m2v70">
                                We look for numbers adding to <m>8</m> and multiplying to <m>15</m>; <m>3</m> and <m>5</m> meet those conditions, so rewrite the middle term:
                                <md>
                                    <mrow>x^2 + 8x + 15 \amp = x^2 + 3x + 5x + 15</mrow>
                                    <mrow>\amp = x(x + 3) + 5(x + 3)</mrow>
                                    <mrow>\amp = (x + 3)(x + 5)</mrow>
                                </md>
                            </p>
                        </li>
                        <li xml:id="auto_jz8m9z2n">
                            <p xml:id="auto_yrc65jxz">
                                We need numbers summing to <m>-7</m> and multiplying to <m>12</m>; <m>-3</m> and <m>-4</m> satisfy this, so split the middle term accordingly:
                                <md>
                                    <mrow>x^2 - 7x + 12 \amp = x^2 - 3x - 4x + 12</mrow>
                                    <mrow>\amp = x(x - 3) - 4(x - 3)</mrow>
                                    <mrow>\amp = (x - 3)(x - 4)</mrow>
                                </md>
                            </p>
                        </li>
                        <li xml:id="auto_zka8y8gt">
                            <p xml:id="auto_01i8tylc">
                                We need numbers that add to <m>-6</m> and multiply to <m>9</m>; <m>-3</m> and <m>-3</m> do, showing this is a perfect square. Splitting the middle term:
                                <md>
                                    <mrow>x^2 - 6x + 9 \amp = x^2 - 3x - 3x + 9</mrow>
                                    <mrow>\amp = x(x - 3) - 3(x - 3)</mrow>
                                    <mrow>\amp = (x - 3)(x - 3)</mrow>
                                </md>
                            </p>
                        </li>
                        <li xml:id="auto_prekbx59">
                            <p xml:id="auto_w9qi5cjf">
                                The numbers must sum to <m>3</m> and multiply to <m>2</m>; <m>1</m> and <m>2</m> satisfy this, so separate the middle term with <m>1x</m> and <m>2x</m>:
                                <md>
                                    <mrow>x^2 + 3x + 2 \amp = x^2 + x + 2x + 2</mrow>
                                    <mrow>\amp = x(x + 1) + 2(x + 1)</mrow>
                                    <mrow>\amp = (x + 1)(x + 2)</mrow>
                                </md>
                            </p>
                        </li>
                        <li xml:id="auto_f272ae6j">
                            <p xml:id="auto_z5coltuc">
                                We need numbers that add to <m>-5</m> and multiply to <m>6</m>; <m>-2</m> and <m>-3</m> work, so use them to rewrite the middle term:
                                <md>
                                    <mrow>x^2 - 5x + 6 \amp = x^2 - 2x - 3x + 6</mrow>
                                    <mrow>\amp = x(x - 2) - 3(x - 2)</mrow>
                                    <mrow>\amp = (x - 2)(x - 3)</mrow>
                                </md>
                            </p>
                        </li>
                        <li xml:id="auto_g59o8z1p">
                            <p xml:id="auto_53y19knp">
                                Find numbers summing to <m>2</m> and multiplying to <m>-15</m>; <m>5</m> and <m>-3</m> fit, so split the middle term with those values:
                                <md>
                                    <mrow>x^2 + 2x - 15 \amp = x^2 + 5x - 3x - 15</mrow>
                                    <mrow>\amp = x(x + 5) - 3(x + 5)</mrow>
                                    <mrow>\amp = (x + 5)(x - 3)</mrow>
                                </md>
                            </p>
                        </li>
                        <li xml:id="auto_16r2p6wp">
                            <p xml:id="auto_abdbe0om">
                                We want numbers adding to <m>-4</m> and multiplying to <m>-5</m>; <m>-5</m> and <m>1</m> work, so express the middle term as <m>-5x + x</m>:
                                <md>
                                    <mrow>x^2 - 4x - 5 \amp = x^2 - 5x + x - 5</mrow>
                                    <mrow>\amp = x(x - 5) + 1(x - 5)</mrow>
                                    <mrow>\amp = (x - 5)(x + 1)</mrow>
                                </md>
                            </p>
                        </li>
                        <li xml:id="auto_xgk2vdaz">
                            <p xml:id="auto_yymjg982">
                                Numbers must total <m>-3</m> and multiply to <m>-10</m>; <m>-5</m> and <m>2</m> meet this, letting us split the middle term:
                                <md>
                                    <mrow>x^2 - 3x - 10 \amp = x^2 - 5x + 2x - 10</mrow>
                                    <mrow>\amp = x(x - 5) + 2(x - 5)</mrow>
                                    <mrow>\amp = (x - 5)(x + 2)</mrow>
                                </md>
                            </p>
                        </li>
                        <li xml:id="auto_4wykv1u9">
                            <p xml:id="auto_eq1qarbq">
                                We need numbers adding to <m>7</m> and multiplying to <m>10</m>; <m>5</m> and <m>2</m> satisfy this, so rewrite the middle term as <m>5x + 2x</m>:
                                <md>
                                    <mrow>x^2 + 7x + 10 \amp = x^2 + 5x + 2x + 10</mrow>
                                    <mrow>\amp = x(x + 5) + 2(x + 5)</mrow>
                                    <mrow>\amp = (x + 5)(x + 2)</mrow>
                                </md>
                            </p>
                        </li>
                        <li xml:id="auto_18xxgfn3">
                            <p xml:id="auto_9kynstyy">
                                We search for numbers summing to <m>-8</m> and multiplying to <m>-20</m>; <m>-10</m> and <m>2</m> work, so split using those:
                                <md>
                                    <mrow>x^2 - 8x - 20 \amp = x^2 - 10x + 2x - 20</mrow>
                                    <mrow>\amp = x(x - 10) + 2(x - 10)</mrow>
                                    <mrow>\amp = (x - 10)(x + 2)</mrow>
                                </md>
                            </p>
                        </li>
                        <li xml:id="auto_1gp0oeru">
                            <p xml:id="auto_gkqh0vao">
                                We need numbers that add to <m>9</m> and multiply to <m>20</m>; <m>4</m> and <m>5</m> work perfectly, so use them to break the middle term:
                                <md>
                                    <mrow>x^2 + 9x + 20 \amp = x^2 + 4x + 5x + 20</mrow>
                                    <mrow>\amp = x(x + 4) + 5(x + 4)</mrow>
                                    <mrow>\amp = (x + 4)(x + 5)</mrow>
                                </md>
                            </p>
                        </li>
                    </ol>
                </p>
            </answer>
        </exercise>
    </exercises>
</subsubsection>